Fix the corelib to use the new syntax with ; (not 𝒰 yet)

theories/extraction/ExtractionSort.v
@@ -6,13 +6,13 @@ Constraint Type ~> Extr.
 Set Universe Polymorphism.
 Set Sort Polymorphism.
 
-Class LargeElimSort@{s t| l l' | t ~> Type , l < l'} : Type@{t|l'+1} :=
-{ Univ : Type@{s|l'} ;
-  code : Type@{s|l} -> Univ ;   
-  El : Univ -> Type@{s|l} ;
-  El_code A : El (code A) = A :> Type@{s|l} }.
+Class LargeElimSort@{s t; l l' | t ~> Type, l < l'} : Type@{t;l'+1} :=
+{ Univ : Type@{s;l'} ;
+  code : Type@{s;l} -> Univ ;   
+  El : Univ -> Type@{s;l} ;
+  El_code A : El (code A) = A :> Type@{s;l} }.
 
-Instance ExtrLargeElimSort@{l l'| l < l'} : LargeElimSort@{Extr Type | l l'}. 
+Instance ExtrLargeElimSort@{l l'| l < l'} : LargeElimSort@{Extr Type; l l'}. 
 Admitted. 
 
 Inductive nat : Type :=
@@ -22,39 +22,39 @@ Inductive nat : Type :=
 Inductive unit : Type := tt.
 Inductive empty : Type := .
 
-Definition nat_rect@{i} := nat_poly@{Type Type | i}.
-Definition nat_rec@{i} := nat_poly@{Type Type | i}.
-Definition nat_ind@{i} := nat_poly@{Type Prop | i}.
-Definition nat_sind@{i} := nat_poly@{Type SProp | i}.
+Definition nat_rect@{i} := nat_poly@{Type Type; i}.
+Definition nat_rec@{i} := nat_poly@{Type Type; i}.
+Definition nat_ind@{i} := nat_poly@{Type Prop; i}.
+Definition nat_sind@{i} := nat_poly@{Type SProp; i}.
 
-Definition P@{s|u u'|u <u'} {H:LargeElimSort@{s Type|u u'}} (n : nat@{s|}) :=
+Definition P@{s;u u'|u <u'} {H:LargeElimSort@{s Type;u u'}} (n : nat@{s;}) :=
   match n return H.(Univ) with
-    O => code unit@{s|u}
-  | _ => code empty@{s|u}
+    O => code unit@{s;u}
+  | _ => code empty@{s;u}
   end.
 
-Lemma eq_true@{s|u u'|u <u'} {H:LargeElimSort@{s Type|u u'}} : forall (n:nat@{s|}), O = n -> H.(El) (P n).
+Lemma eq_true@{s;u u'|u <u'} {H:LargeElimSort@{s Type;u u'}} : forall (n:nat@{s;}), O = n -> H.(El) (P n).
 Proof.
-  intros b e. destruct e. cbn. eapply (eq_poly _ (fun X => X) tt _ (eq_sym@{Type s|_ _} (H.(El_code) unit))).
+  intros b e. destruct e. cbn. eapply (eq_poly _ (fun X => X) tt _ (eq_sym@{Type s;_ _} (H.(El_code) unit))).
 Qed.
 
-Lemma nat_discr@{s|u u'|u <u'} {H:LargeElimSort@{s Type|u u'}} (n : nat@{s|}): O = S n -> empty@{s|u}.
+Lemma nat_discr@{s;u u'|u <u'} {H:LargeElimSort@{s Type;u u'}} (n : nat@{s;}): O = S n -> empty@{s;u}.
 Proof.
   intro e. pose proof (eq_true _ e). eapply (eq_poly _ (fun X => X) X _ (H.(El_code) _)).
 Qed.
 
-Lemma nat_discr_extr (n : nat@{Extr|}): O = S n -> False.
+Lemma nat_discr_extr (n : nat@{Extr;}): O = S n -> False.
 Proof.
   intro e. pose proof (nat_discr n e). destruct X.
 Qed.  
 
-Inductive Vect (A : Type) : nat@{Extr|} -> Type :=
+Inductive Vect (A : Type) : nat@{Extr;} -> Type :=
 | vnil : Vect A O
 | vcons : forall (a:A) n, Vect A n -> Vect A (S n).
 
-Fail Definition length A n : Vect A n -> nat@{Type|} := fun _ => n. 
+Fail Definition length A n : Vect A n -> nat@{Type;} := fun _ => n. 
 
-Fixpoint length A n : Vect A n -> nat@{Type|} := 
+Fixpoint length A n : Vect A n -> nat@{Type;} := 
   fun v => match v with 
     | vnil _ => O 
     | vcons _  a n v => S (length A n v)
