theories/Classes/CMorphisms.v
@@ -590,7 +590,7 @@ Section Normalize.
 
   Lemma proper_normalizes_proper `(Normalizes R0 R1, Proper A R1 m) : Proper R0 m.
   Proof.
-    edestruct H. eapply r0. assumption.
+    edestruct H as [r r']. eapply r'. assumption.
   Qed.
 
   Lemma flip_atom R : Normalizes R (flip (flip R)).
@@ -710,7 +710,7 @@ split; compute.
     apply Hxy'.
     apply partial_order_antisym; auto.
     apply transitivity with z; [assumption|].
-    destruct (H x z). destruct r; eauto.
+    destruct (H x z) as [r r']. destruct r; eauto.
 Qed.
 
 (** From a [StrictOrder] to the corresponding [PartialOrder]:
@@ -727,9 +727,9 @@ split.
   + left. apply transitivity with y; auto.
   + left. eapply H1; try eassumption. apply reflexivity.
   + left. eapply H1 with y z; [now apply symmetry|apply reflexivity|try eassumption].
-  + right. apply transitivity with y; auto.
-  
-  Qed.*) Admitted.
+  + right. apply transitivity with y; auto.  
+Qed.
+
 #[global]
 Hint Extern 4 (PreOrder (relation_disjunction _ _)) => 
     class_apply StrictOrder_PreOrder : typeclass_instances.
@@ -741,11 +741,9 @@ Proof.
 intros. intros x y. compute. intuition auto.
 - right; now apply symmetry.
 - elim (StrictOrder_Irreflexive x).
-  eapply transitivity with y; eauto. 
-  (*  
+  eapply transitivity with y; eauto.     
 - now apply symmetry.
-Qed.*)
-Admitted.
+Qed.
 
 #[global]
 Hint Extern 4 (StrictOrder (relation_conjunction _ _)) => 
